Adds encodings for section 3

Background.v
@@ -1,6 +1,159 @@
-Require Import Coq.Program.Basics. 
+Require Import Program.Basics.
+Require Import FunctionalExtensionality.
 
 Open Scope program_scope.
+
+
+(***************)
+(* Typeclasses *)
+(***************)
+
+(* Monad *)
+
+Class Monad (m : Type -> Type) : Type :=
+{ ret : forall {X}, X -> m X
+; bind : forall {A B}, m A -> (A -> m B) -> m B
+}.
+Notation "ma >>= f" := (bind ma f) (at level 50, left associativity).
+Notation "ma >> mb" := (ma >>= fun _ => mb) (at level 50, left associativity).
+
+Class MonadLaws (m : Type -> Type) `{Monad m} :=
+{ left_id : forall {A B} (a : A) (f : A -> m B), ret a >>= f = f a
+; right_id : forall {A} (ma : m A), ma >>= ret = ma
+; assoc : forall {A B C} (ma : m A) (f : A -> m B) (g : B -> m C),
+                 ma >>= f >>= g = ma >>= (fun x => f x >>= g)
+}.
+
+(* MonadState *)
+
+Class MonadState (A : Type) (m : Type -> Type) `{Monad m} :=
+{ get : m A
+; put : A -> m unit
+; modify : (A -> A) -> m unit := fun f => get >>= (put ∘ f)
+}.
+
+Class MonadStateLaws (A : Type) (m : Type -> Type) `{MonadState A m} :=
+{ get_get : get >>= (fun s1 => get >>= (fun s2 => ret (s1, s2))) =
+            get >>= (fun s => ret (s, s))
+; get_put : get >>= put = ret tt
+; put_get : forall s, put s >> get = put s >> ret s
+; put_put : forall s1 s2, put s1 >> put s2 = put s2
+}.
+
+Ltac unwrap_layer := 
+  apply f_equal;
+  apply functional_extensionality;
+  intros.
+
+Lemma general_getget : 
+    forall {M : Type -> Type} {A : Type}
+          `{MSL : MonadStateLaws A M} {ML : MonadLaws M} {X : Type} 
+           (p : A * A -> M X),
+           get >>= (fun x1 => get >>= (fun x2 => p (x1, x2))) = 
+           get >>= (fun x1 => p (x1, x1)).
+Proof.
+  intros.
+  destruct ML.
+  destruct MSL.
+  assert (G : get >>= (fun x1 : A => p (x1, x1)) =
+              get >>= (fun x1 : A => ret (x1, x1) >>= p)).
+  { unwrap_layer. now rewrite left_id0. }
+  rewrite G.
+  rewrite <- assoc0.
+  rewrite <- get_get0.
+  rewrite -> assoc0.
+  unwrap_layer.
+  rewrite -> assoc0.
+  unwrap_layer.
+  now rewrite left_id0.
+Qed.
+
+Lemma non_eff_get : 
+    forall  {m : Type -> Type} {A : Type}
+           `{M : Monad m}
+            {ML : @MonadLaws m M}
+            {MS : @MonadState A m M}
+            {MSL : @MonadStateLaws A m M MS} {X : Type} (p : m X),
+    get >> p = p.
+Proof.
+  intros.
+  pose proof (@general_getget m A M MS MSL ML) as J.
+  destruct ML.
+  destruct MSL.
+  rewrite <- (left_id0 unit _ tt (fun _ => p)).
+  rewrite <- get_put0.
+  repeat rewrite assoc0.
+  now rewrite (J X (fun pair => put (snd pair) >> p)).
+Qed.
+
+
+(*********)
+(* State *)
+(*********)
+
+Record state (S A : Type) := mkState
+{ runState : S -> A * S }.
+Arguments mkState [S A].
+Arguments runState [S A].
+
+Definition evalState {S A} (st : state S A) (s : S) : A :=
+  fst (runState st s).
+
+Definition execState {S A} (st : state S A) (s : S) : S :=
+  snd (runState st s).
+
+Ltac state_reason :=
+  match goal with
+  | [ |- context [bind _]] => unfold bind
+  | [ |- context [execState] ] => unfold execState
+  | [ |- context [evalState] ] => unfold evalState
+  | [ |- {| runState := _ |} = {| runState := _ |} ] => apply f_equal
+  | [ |- (fun _ => _) = _ ] => apply functional_extensionality; intros
+  | [ |- {| runState := _ |} = ?x ] => destruct x as [rs]
+  | [ |- context [ let (_, _) := ?rs ?x in _ ] ] => destruct (rs x)
+  end; simpl; auto.
+
+Ltac i_state_reason := intros; repeat state_reason.
+
+Instance Monad_state {S : Type} : Monad (state S) :=
+{ ret := fun X x => mkState (fun s => (x, s))
+; bind := fun A B m f => mkState (fun s => let (a, s') := runState m s
+                                           in runState (f a) s')
+}.
+
+Instance MonadLaws_state {S : Type} : MonadLaws (state S).
+Proof.
+  constructor; intros; repeat state_reason.
+Qed.
+
+Instance MonadState_state {S : Type} : MonadState S (state S) :=
+{ get := mkState (fun s => (s, s))
+; put := fun s => mkState (fun _ => (tt, s))
+}.
+
+Instance MonadStateLaws_state {S : Type} : MonadStateLaws S (state S).
+Proof. constructor; auto. Qed.
+
+Lemma execexec_is_execgtgt : 
+    forall {S A B} (s : S) (st1 : state S A) (st2 : state S B),
+           execState st2 (execState st1 s) = execState (st1 >> st2) s.
+Proof. i_state_reason. Qed.
+
+Lemma execeval_is_evalgtgt :
+    forall {S A B} (s : S) (st1 : state S A) (st2 : state S B),
+           evalState st2 (execState st1 s) = evalState (st1 >> st2) s.
+Proof. i_state_reason. Qed.
+
+Lemma execevalexec_is_execbind :
+    forall {S A B} (s : S) (st1 : state S A) (f : A -> state S B),
+           execState (f (evalState st1 s)) (execState st1 s) = 
+           execState (st1 >>= f) s.
+Proof. i_state_reason. Qed.
+
+Lemma eval_ma_gtgt_retx_is_x : 
+    forall {S A X} (m : state S A) (s : S) (x : X),
+           evalState (m >> ret x) s = x.
+Proof. i_state_reason. Qed.
 
 
 (**********)
@@ -17,6 +170,21 @@ Arguments mkLens [S A].
 Arguments view [S A].
 Arguments update [S A].
 
+Definition view_update {S A : Type} (ln : lens S A) : Prop :=
+  forall s, update ln s (view ln s) = s.
+
+Definition update_view {S A : Type} (ln : lens S A) : Prop :=
+  forall s a, view ln (update ln s a) = a.
+
+Definition well_behaved {S A : Type} (ln : lens S A) : Prop :=
+  view_update ln /\ update_view ln.
+
+Definition update_update {S A : Type} (ln : lens S A) : Prop :=
+  forall s a1 a2, update ln (update ln s a1) a2 = update ln s a2.
+
+Definition very_well_behaved {S A : Type} (ln : lens S A) : Prop :=
+  well_behaved ln /\ update_update ln.
+
 Definition composeLn {S A B} (ln1 : lens S A) (ln2 : lens A B) : lens S B := 
   mkLens ((view ln2) ∘ (view ln1)) 
          (fun s => update ln1 s ∘ update ln2 (view ln1 s)).
@@ -25,6 +193,9 @@ Notation "ln1 ▷ ln2" := (composeLn ln1 ln2) (at level 40, left associativity).
 Definition modifyLn {S A} (ln : lens S A) (f : A -> A) : S -> S :=
   fun s => update ln s (f (view ln s)).
 Notation "ln %~ f" := (modifyLn ln f) (at level 40, no associativity).
+
+Definition identityLn A : lens A A := 
+  mkLens id (fun _ => id).
 
 
 (* Prism datatype and definitions *)
@@ -68,38 +239,3 @@ Definition composeLnPr {S A B} (ln : lens S A) (pr : prism A B) : affine S B :=
                        | none => s
                        end).
 Notation "ln ▶ pr" := (composeLnPr ln pr) (at level 40, left associativity).
-
-
-(***************)
-(* Typeclasses *)
-(***************)
-
-(* Monad *)
-
-(* Pattern to describe `Monad` laws with a nicer notation *)
-Class monad_bind (m : Type -> Type) := 
-  monad_bind_ : forall {A B}, m A -> (A -> m B) -> m B.
-Notation "ma >>= f" := (monad_bind_ ma f) (at level 50, left associativity).
-Notation "ma >> mb" := (ma >>= fun _ => mb) (at level 50, left associativity).
-
-Class Monad (m : Type -> Type)
-            (bind : monad_bind m) : Type :=
-{ ret : forall {A}, A -> m A
-; left_id : forall {A B} (a : A) (f : A -> m B), ret a >>= f = f a
-; right_id : forall {A} (ma : m A), ma >>= ret = ma
-; assoc : forall {A B C} (ma : m A) (f : A -> m B) (g : B -> m C),
-                 ma >>= f >>= g = ma >>= (fun x => f x >>= g)
-}.
-
-
-(* MonadState *)
-
-Class MonadState (A : Type) (m : Type -> Type) `{Monad m} :=
-{ get : m A
-; put : A -> m unit
-; get_get : get >>= (fun s1 => get >>= (fun s2 => ret (s1, s2))) =
-            get >>= (fun s => ret (s, s))
-; get_put : get >>= put = ret tt
-; put_get : forall s, put s >> get = put s >> ret s
-; put_put : forall s1 s2, put s1 >> put s2 = put s2
-}.
