Towards.v
@@ -1,0 +1,109 @@
+Require Import Coq.Program.Basics. 
+Require Import Strings.String.
+Require Import Background.
+
+
+(* `MonadState` generalizes `lens` *)
+
+Definition MonadState_state_2_lens A : lens A A :=
+  mkLens (fun a => evalState get a) (fun a a' => execState (put a') a).
+
+Lemma MonadState_state_is_identity_lens : forall A,
+    MonadState_state_2_lens A = identityLn A.
+Proof. auto. Qed.
+
+Definition ms_2_lens {S A} (ms : MonadState A (state S)) : lens S A :=
+{| view s     := evalState get s
+;  update s a := execState (put a) s
+|}.
+
+Instance lens_2_ms {S A} (ln : lens S A) : MonadState A (state S) :=
+{ get   := mkState (fun s => (view ln s, s))
+; put a := mkState (fun s => (tt, update ln s a))
+}.
+
+Ltac i_unfold_behavedness :=
+  unfold very_well_behaved; unfold well_behaved; 
+  unfold view_update; unfold update_view; unfold update_update;
+  unfold get; unfold put;
+  unfold ms_2_lens; unfold lens_2_ms;
+  intros.
+
+Theorem MonadState_state_s_induces_lens : 
+    forall {S A : Type} (ms : MonadState A (state S)),
+           @MonadStateLaws A (state S) _ ms -> very_well_behaved (ms_2_lens ms).
+Proof.
+  i_unfold_behavedness.
+  assert (F : forall s, put (evalState get s) = get >> put (evalState get s)).
+  { intros.
+    rewrite <- (non_eff_get (put (evalState get s))).
+    now rewrite (general_getget (fun _ => put (evalState get s))). }
+  destruct H.
+  repeat split; intros; simpl.
+
+  - (* view_update *)
+    rewrite F.
+    rewrite <- execexec_is_execgtgt.
+    rewrite execevalexec_is_execbind.
+    now rewrite get_put.
+
+  - (* update_view *)
+    rewrite execeval_is_evalgtgt.
+    rewrite put_get.
+    now rewrite eval_ma_gtgt_retx_is_x.
+
+  - (* updte_update *)
+    rewrite execexec_is_execgtgt.
+    now rewrite put_put.
+Qed.
+
+Theorem lens_induces_MonadState_state_s :
+    forall {S A : Type} (ln : lens S A),
+           very_well_behaved ln -> @MonadStateLaws A (state S) _ (lens_2_ms ln).
+Proof.
+  i_unfold_behavedness.
+  destruct H as [[view_update update_view] update_update].
+  split; 
+    simpl; 
+    intros; 
+    repeat state_reason; 
+    [rewrite view_update | rewrite update_view | rewrite update_update];
+    auto.
+Qed.
+
+
+(* Lens Algebra definition *)
+
+Record lensAlg (p : Type -> Type) (A : Type) `{M : Monad p} : Type :=
+{ (* abstract definitions *)
+  get : p A
+; put : A -> p unit
+
+  (* laws *)
+; get_get : get >>= (fun s1 => get >>= (fun s2 => ret (s1, s2))) =
+            get >>= (fun s => ret (s, s))
+; get_put : get >>= put = ret tt
+; put_get : forall s, put s >> get = put s >> ret s
+; put_put : forall s1 s2, put s1 >> put s2 = put s2
+
+  (* derived methods *)
+; modify (f : A -> A) : p unit := get >>= (put ∘ f)
+}.
+Arguments get [p A _].
+Arguments put [p A _].
+Arguments modify [p A _].
+
+
+(* Zip example *)
+
+Class Address'' (p : Type -> Type) `{Monad p} :=
+{ zip'' : lensAlg p nat
+; getRegion'' : p (option string)
+; modRegion'' (f : string -> string) : p unit
+}.
+
+Definition modifyZip (f : nat -> nat) {p} `{Address'' p} : p unit :=
+  modify zip'' f.
+
+Definition getZip {p} `{Address'' p} : p nat :=
+  get zip''.
